Capless/Subst/Term/CaptureBound.lean
@@ -1,0 +1,42 @@
+import Capless.CaptureBound
+import Capless.Subst.Basic
+import Capless.Subst.Term.Subcapturing
+
+/-
+Substitution theorems for term variable substitution in capture kind judgments.
+-/
+
+namespace Capless
+
+theorem CaptureKind.subst
+  (h : CaptureKind Γ C K)
+  (σ : VarSubst Γ f Δ) :
+  CaptureKind Δ (C.rename f) K := by
+  induction h
+  case var hb hk ih =>
+    have hb1 := σ.map _ _ hb
+    simp [EType.rename, CType.rename] at hb1
+    have h := Typing.inv_subcapt hb1
+    apply csub h (ih σ)
+  case cvar hb =>
+    have hb1 := σ.cmap _ _ hb
+    apply cvar hb1
+  case csub hsub hk ih =>
+    have hsub1 := hsub.subst σ
+    apply csub hsub1 (ih σ)
+  case sub hs hk ih =>
+    apply sub hs (ih σ)
+  case union h1 h2 ih1 ih2 =>
+    apply union (ih1 σ) (ih2 σ)
+  case empty =>
+    apply empty
+
+theorem CaptureBound.subst
+  (h : CaptureBound Γ C B)
+  (σ: VarSubst Γ f Δ) :
+  CaptureBound Δ (C.rename f) (B.rename f) := by
+    cases h <;> constructor
+    apply Subcapt.subst _ σ ; assumption
+    apply CaptureKind.subst _ σ ; assumption
+
+end Capless
