Capless/Subst/Type/CaptureBound.lean
@@ -1,0 +1,41 @@
+import Capless.CaptureBound
+import Capless.Subst.Basic
+import Capless.Subst.Type.Subcapturing
+
+/-
+Substitution theorems for type variable substitution in capture kind judgments.
+-/
+
+namespace Capless
+
+theorem CaptureKind.tsubst
+  (h : CaptureKind Γ C K)
+  (σ : TVarSubst Γ f Δ) :
+  CaptureKind Δ C K := by
+  induction h
+  case var hb hk ih =>
+    have hb1 := σ.map _ _ hb
+    simp [CType.trename] at hb1
+    apply var hb1 (ih σ)
+  case cvar hb =>
+    have hb1 := σ.cmap _ _ hb
+    apply cvar hb1
+  case csub hsub hk ih =>
+    have hsub1 := hsub.tsubst σ
+    apply csub hsub1 (ih σ)
+  case sub hs hk ih =>
+    apply sub hs (ih σ)
+  case union h1 h2 ih1 ih2 =>
+    apply union (ih1 σ) (ih2 σ)
+  case empty =>
+    apply empty
+
+theorem CaptureBound.tsubst
+  (h : CaptureBound Γ C B)
+  (σ: TVarSubst Γ f Δ) :
+  CaptureBound Δ C B := by
+    cases h <;> constructor
+    apply Subcapt.tsubst _ σ ; assumption
+    apply CaptureKind.tsubst _ σ ; assumption
+
+end Capless
