Capless/Weakening/CaptureBound.lean
@@ -1,0 +1,22 @@
+import Capless.CaptureBound
+import Capless.Weakening.Basic
+import Capless.Renaming.Term.CaptureBound
+import Capless.Renaming.Type.CaptureBound
+import Capless.Renaming.Capture.CaptureBound
+
+namespace Capless
+
+def CaptureKind.weaken
+  (h : CaptureKind Γ C K) :
+   CaptureKind (Γ,x: T) C.weaken K := by
+  apply h.rename VarMap.weaken
+
+def CaptureKind.tweaken
+  (h : CaptureKind Γ C K) :
+  CaptureKind (Γ.tvar b) C K := by
+  apply h.trename TVarMap.weaken
+
+def CaptureKind.cweaken
+  (h : CaptureKind Γ C K) :
+  CaptureKind (Γ.cvar b) C.cweaken K := by
+  apply h.crename CVarMap.weaken
